cleanup / rearranging

generic.v
@@ -9,21 +9,8 @@ Require Import univ utils.
 
 (* Generic Library *)
 
-(** Still mostly just playing around, this is basically a combination of ideas
-  from 'Arity-Generic Datatype-Generic Programming' and
-  'Polytypic Programming in Coq'. **)
-
 (****** Type specialization ******)
 
-(** "The type of a generic function instance from four pieces of information:
-    - the arity of the operation, given with an implicit argument n
-    - a function b to construct the type in the base case
-    - the kind k itself
-    - a vector v of n Coq types, each of kind k" *)
-
-(* so b is literally the way to construct the type of the operation
-      e.g. Map : vec Set 2 -> Set
-      Map (A :: B :: []) = A -> B *)
 Fixpoint kit (n : nat) (k : kind) (b : vec Type (S n) -> Type)
   : vec (decodeKind k) (S n) -> Type :=
     match k return vec (decodeKind k) (S n) -> Type with
@@ -46,41 +33,6 @@ Fixpoint unkit (n : nat) (k : kind) (b : vec Type (S n) -> Type)
 Definition tyConstEnv (n : nat) (b : vec Type (S n) -> Type) : Type :=
   forall (k:kind) (c:const k), kit k b (repeat _ (decodeClosed (Con _ c))).
 
-Section cmap.
-  (* An example of defining constants for map *)
-
-  (* type for the operation aka: [a,b] to (a -> b) *)
-  Definition Map : vec Type 2 -> Type :=
-    fun vs => vhd vs -> vhd (vtl vs).
-
-  (* helper for mapConst *)
-  Definition doSum (A1 B1 : Type)
-    : (A1 -> B1) -> forall (A2 B2 : Type), (A2 -> B2) -> (A1 + A2) -> (B1 + B2) :=
-    fun f =>
-      fun _ _ g sa =>
-        match sa with
-        | inl a => inl (f a)
-        | inr b => inr (g b)
-        end.
-
-  (* helper for mapConst *)
-  Definition doProd (A1 B1 : Type)
-    : (A1 -> B1) -> forall (A2 B2 : Type), (A2 -> B2) -> (A1 * A2) -> (B1 * B2) :=
-    fun f _ _ g sa => (f (fst sa), g (snd sa)).
-
-  (* Example of building a function for mapping constants to a value. *)
-  Definition mapConst : tyConstEnv Map :=
-    fun k c =>
-      match c in const k
-      return kit k Map (repeat _ (decodeClosed (Con _ c)))
-      with
-      | Nat => fun n => n
-      | Unit => fun _ => tt
-      | Prod => doProd
-      | Sum => doSum
-      end.
-End cmap.
-
 (* Now what is left is term specialization and then done for type-genericity *)
 
 Section terms.
@@ -97,24 +49,6 @@ Section terms.
     : typ G k -> vec (env G) n -> vec (decodeKind k) n :=
     fun t vs =>
       zap (repeat _ (decodeType t)) vs.
-
-  Lemma zr : forall n G k (t1 : tyvar G k) (a : env G) (v : vec (env G) n),
-    zap (repeat (S n) (decodeType (Var t1))) (vcons a v)
-    = vcons (decodeType (Var t1) a)
-    (zap (repeat n (decodeType (Var t1))) v).
-  Proof.
-    intros. reflexivity.
-  Defined.
-
-  Lemma ineqv : forall n G k (t1 t2 : tyvar G k) (v : vec (env G) n),
-    interp' (Var t1) v = interp' (Var t2) v.
-  Proof.
-    intros.
-    intros. induction v.
-    - destruct t1; reflexivity.
-    - unfold interp'. unfold interp' in IHv. rewrite zr. rewrite zr.
-      rewrite IHv. simpl.
-  Admitted.
 
   (* kit equality *)
   Definition eqkit : forall (n : nat) (k : kind) (b : vec Type (S n) -> Type)
@@ -226,20 +160,10 @@ Section terms.
     - apply eqtail. apply IHa.
   Defined.
 
-(*
-  Import EqNotations.
-
-   https://jamesrwilcox.com/dep-destruct.html 
-  Lemma inv (k k' : kind) (G : ctx) (v : tyvar (k' :: G) k) :
-    {p : k' = k | rew [fun k' : kind => tyvar (k' :: G) k] p in v = Vz G k} +
-    {w : tyvar G k | v = Vs k' w}.
-  Proof.
-    pattern v. apply tvcase; intros.
-    - left. apply exist with (x:=eq_sym pf). subst; auto.
-    - right. apply exist with (x:=x). reflexivity.
-  Defined.*)
-
-  (* Lookup a type for var from nge  *)
+  (** Lookup a type for var from nge.
+      Requires a self defined lemma 'tvcase' for destructing v.
+      Done following the idea presented by James Wilcox in:
+      - https://jamesrwilcox.com/dep-destruct.html              **)
   Fixpoint nlookup (n : nat) (k : kind) (b : vec Type (S n) -> Type) (G : ctx)
     (v : tyvar G k) (nge : ngenv b G) :
     kit k b (interp' (Var v) (transpose nge)).
@@ -255,20 +179,6 @@ Section terms.
         apply eqkit with (b:=b) in ch.
         * apply ch.
        * exact (nlookup _ _ _ _ x nge). Defined.
-
-         (*
-    - pose proof inv v as i. destruct i as [[p e] | [w e]].
-      + subst. apply eqkit with (t1 := a).
-        * pose proof (c1 _ a (transpose nge)) as ch. simpl in ch. simpl.
-          cbn in e. rewrite e.
-          rewrite <- ch. reflexivity.
-        * apply k1.
-      + rewrite e.
-        pose proof (c2 _ w a (transpose nge)) as ch.
-        apply eqkit with (b:=b) in ch.
-        * apply ch.
-       * exact (nlookup _ _ _ _ w nge). Defined.
-         *)
 
   (* term specialization with non-empty context *)
   Fixpoint ngen' (n : nat) (b : vec Type (S n) -> Type)
@@ -300,323 +210,37 @@ Section terms.
 
 End terms.
 
-(* Now we can use ngen and mapConst to define a generic map *)
+(* mb smth ?
+Record NGen : Type := mkNGen
+  {
+    transform : forall n, vec Type (S n) -> Type;
+    cnat : forall n,
+      kit Ty (@transform n) (repeat (S n) (decodeClosed (Con [] Nat)));
+    cunit : forall n,
+      kit Ty (@transform n) (repeat (S n) (decodeClosed (Con [] Unit)));
+    csum : forall n,
+      kit (F Ty (F Ty Ty)) (@transform n) (repeat (S n) (decodeClosed (Con [] Sum)));
+    cprod : forall n,
+      kit (F Ty (F Ty Ty)) (@transform n) (repeat (S n) (decodeClosed (Con [] Prod)));
+    ngconst : forall n,
+      tyConstEnv (@transform n)
+  }.
 
-Definition gmap (k : kind) (t : ty k) : kit k Map _ :=
-  ngen t mapConst.
+Program Definition ng := mkNGen
+  (@funTy)
+  _
+  _
+  _
+  _
+  _.
+Next Obligation.
+  induction n.
+  - apply 0.
+  - simpl; intros. apply IHn. Defined.
+Next Obligation. Admitted.
+Next Obligation. Admitted.
+Next Obligation. Admitted.
+Next Obligation. Admitted.
 
-(* examples  of using gmap *)
-Compute gmap tprod nat nat (fun a => a + 1) bool bool (fun b => negb b) (1,true).
-(* tmaybe is a self defined type, definition in 'univ.v' *)
-Compute gmap tmaybe _ bool (fun _ => false) (inl tt). (* = inl () *)
-Compute gmap tmaybe nat nat (fun n => n + 1) (inr 3). (* = inr 4 *)
-(* teither is a self defined type, definition in 'univ.v' *)
-Compute gmap teither _ bool (fun _ => false)
-                     _ bool (fun _ => true) (inl tt). (* = inl false *)
+       *)
 
-(***********************************************************************)
-(* with these datatype-genericity done, now just need to add arity-gen *)
-(***********************************************************************)
-
-(* turn a vector of types into a function type, e.g [a,b,c] into: a -> b -> c *)
-Fixpoint funTy {n : nat} (v : vec Type (S n)) : Type :=
-  match v with
-  | @vcons _ O x xs => x
-  | @vcons _ (S n') x xs => x -> funTy xs
-  end.
-
-Section argm.
-  (* example of the functionality that the user needs to provide *)
-  (* aka how doubly-generic map works for constants *)
-
-  (* nat constant for nmapconst *)
-  Fixpoint cNat (n : nat) : kit Ty funTy (repeat (S n) _) :=
-    let f := (fix cNat' (n' : nat)
-      : kit Ty funTy (repeat (S n') nat) :=
-      match n' return kit Ty funTy (repeat (S n') nat) with
-      | O => O
-      | S O => fun x => x
-      | S (S m) => fun x y => cNat' m
-    end) in
-    match n return kit Ty funTy (repeat (S n) nat) with
-    | O => O
-    | S O => fun x => x
-    | (S (S m)) =>
-        if Nat.odd m
-        then fun x y => cNat m
-        else fun x => f (S m)
-    end.
-
-  (* unit constant for nmapconst *)
-  Fixpoint cUnit (n : nat) : kit Ty funTy (repeat (S n) _) :=
-    match n with
-    | O => tt
-    | S n' => fun x => cUnit n'
-    end.
-
-  (* Error axiom for finishing defs in sums *)
-  Axiom error : False.
-
-  (* helpers for defining sums *)
-  Fixpoint hSumLeft (n : nat)
-    : forall (va : vec Type (S n)), funTy va ->
-    forall (vb : vec Type (S n)), funTy (zap (zap (repeat _ sum) va) vb).
-  Proof.
-    intros VA a VB. simpl.
-    pose proof veq_hdtl VA as pfa;
-    pose proof veq_hdtl VB as pfb.
-    destruct n as [| n'].
-    - rewrite pfa in a. apply (inl a).
-    - intros x. destruct x.
-      + rewrite pfa in a. simpl in a.
-        pose proof a v as pa.
-        pose proof hSumLeft _ _ pa (vtl VB) as pf.
-        apply pf.
-      + pose proof error as err. exfalso; apply err.
-  Defined.
-
-  Fixpoint hSumRight (n : nat)
-    : forall (va : vec Type (S n)) (vb : vec Type (S n)),
-    funTy vb -> funTy (zap (zap (repeat _ sum) va) vb).
-  Proof.
-    intros VA VB b. pose proof veq_hdtl VB as pfb.
-    destruct n as [| n'].
-    - rewrite pfb in b. apply (inr b).
-    - intros x; destruct x as [left | right].
-      + exfalso; apply error.
-      + rewrite pfb in b. simpl in b.
-        pose proof b right as pb.
-        pose proof hSumRight n' (vtl VA)  (vtl VB) pb  as pf.
-        apply pf.
-  Defined.
-
-  Definition hSum (n : nat)
-    : forall (va : vec Type (S n)), funTy va
-    -> forall (vb : vec Type (S n)), funTy vb
-    -> funTy (zap (zap (repeat _ sum) va) vb).
-  Proof.
-    intros VA a VB b.
-    destruct n as [| n'].
-    (* no arguments, chooses arbitrary case inr *)
-    - simpl. rewrite veq_hdtl in b. simpl in b. apply (inr b).
-    - intros x; destruct x as [lr | rt].
-      + rewrite veq_hdtl in a. simpl in a.
-        pose proof a lr as pfa.
-        apply hSumLeft; apply pfa.
-      + rewrite veq_hdtl in b. simpl in b.
-        pose proof b rt as pfb.
-        apply hSumRight; apply pfb.
- Defined.
-
-  (* sum constant for nmapconst *)
-  Definition cSum (n : nat) : kit (F Ty (F Ty Ty)) funTy (repeat (S n) sum).
-  Proof.
-  Admitted.
-
-  Program Fixpoint kindCurry (k : kind) (n : nat) (b : vec Type (S n) -> Type)
-    : forall v : vec (decodeKind k) (S n),
-    unkit k b v -> kit k b v :=
-    match k
-    return forall v : vec (decodeKind k) (S n),
-    unkit k b v -> kit k b v
-    with
-    | Ty => _
-    | F k1 k2 => fun v vs =>
-        curry (fun (x:vec (decodeKind k1) _) =>
-              kit k1 b x ->
-              kit k2 b (zap v x))
-              (fun As y => kindCurry k2 _ (zap v As) (vs As y))
-    end.
-
-  (* [a, b], [c,d] => [(a, c)], [(b, d)] => (a, c) -> (b, d) *)
-
-  (* no fucking clue if correct dadadaaa *)
-  Fixpoint hProd (n : nat)
-    : forall (va : vec Type (S n)), funTy va
-    -> forall (vb : vec Type (S n)), funTy vb
-    -> funTy (zap (zap (repeat _ prod) va) vb).
-      Proof.
-        destruct n;
-        intros VA a VB b;
-        pose proof veq_hdtl VA as pfa;
-        pose proof veq_hdtl VB as pfb.
-        - apply pair.
-          + rewrite pfa in a; apply a.
-          + rewrite pfb in b; apply b.
-        - refine (fun pr => _). intros.
-          destruct pr as [pa pb].
-          apply hProd.
-          + rewrite pfa in a. apply a. apply pa.
-          + rewrite pfb in b. apply b. apply pb.
-      Defined.
-
-  (* prod constant for nmapconst *)
-  Fixpoint cProd (n : nat) : kit (F Ty (F Ty Ty)) funTy (repeat (S n) prod).
-  Proof.
-    apply (kindCurry (F Ty (F Ty Ty))).
-    simpl. intros VA a VB b.
-    pose proof hProd VA a VB b as hp.
-    simpl in hp.
-    apply hp.
-  Defined.
-
-  Fixpoint nmapConst {n : nat} : tyConstEnv (@funTy n).
-  refine (fun k c => _).
-  refine
-  (match c with
-    | Nat => _
-    | Unit => _
-    | Prod => _
-    | Sum => _
-    end
-  ).
-  (* this just returns 0 for all,
-     maybe change to return last nat given (like cNat) *)
-  - induction n.
-    + simpl. apply (cNat 0).
-    + refine (fun x => _). apply IHn.
-  - induction n.
-    + apply tt.
-    + refine (fun x => _). apply IHn.
-  - pose proof (kindCurry (F Ty (F Ty Ty))) as pf.
-    apply pf. simpl. intros VA a VB b.
-    pose proof hSum VA a VB b as hp. simpl in hp.
-    apply hp.
-  - pose proof (kindCurry (F Ty (F Ty Ty))) as pf.
-    apply pf. simpl. intros VA a VB b.
-    pose proof hProd VA a VB b as hp. simpl in hp.
-    apply hp.
-  Defined.
-
-End argm.
-
-Section eq.
-  (* An example of building a doubly-generic equality function *)
-
-  Fixpoint geq {n : nat} (v : vec Type (S n)) : Type :=
-    match v with
-    | @vcons _ O x _ => x -> bool
-    | @vcons _ (S m) x xs => x -> geq xs
-    end.
-
-  Fixpoint geqFalse (n : nat) (v : vec Set (S n)) : geq v :=
-    match v in vec _ (S n) return geq v with
-    | @vcons _ O x _ => fun _ => false
-    | @vcons _ (S m) x xs => fun _ => geqFalse xs
-    end.
-
-  Program Fixpoint eqNat (n : nat) {measure n} : kit Ty geq (repeat (S n) nat) :=
-    match n with
-    | O => fun _ => true
-    | S O => fun a b => Nat.eqb a b
-    | S (S m) => fun a b =>
-        if Nat.eqb a b then eqNat (S m) b
-                       else geqFalse (repeat _ nat)
-    end.
-
-  Fixpoint eqUnit (n : nat) : kit Ty geq (repeat (S n) unit) :=
-    match n with
-    | O => fun _ => true
-    | S n' => fun _ => eqUnit n'
-    end.
-
-  Fixpoint heqProd (n : nat)
-    : forall (va : vec Type (S n)), geq va
-    -> forall (vb : vec Type (S n)), geq vb
-    -> geq (zap (zap (repeat _ prod) va) vb).
-  Proof.
-    intros. destruct n.
-    - simpl. refine (fun pr => _).
-      apply true.
-    - simpl; intros pr. destruct pr as [a b].
-      apply heqProd.
-  Admitted.
-
-  Definition heqSum (n : nat)
-    : forall (va : vec Type (S n)), geq va
-    -> forall (vb : vec Type (S n)), geq vb
-    -> geq (zap (zap (repeat _ sum) va) vb).
-  Proof. Admitted.
-
-  (* sum constant for neqconst  *)
-  Fixpoint eqProd (n : nat) : kit (F Ty (F Ty Ty)) geq (repeat (S n) prod). Admitted.
-
-  Definition eqSum (n : nat) : kit (F Ty (F Ty Ty)) geq (repeat (S n) sum).
-  Admitted.
-
-  (*
-  Program Fixpoint neqConst {n : nat} : tyConstEnv (@geq n) :=
-    fun k c =>
-      match c in const k
-      with
-      (*in const k return kit _ Map (repeat _ (decodeClosed (Con _ c))) with *)
-      | Nat => eqNat _
-      | Unit => eqUnit _
-      | Prod => eqProd _
-      | Sum => eqSum _
-      end.
-      *)
-
-End eq.
-
-(* Now can define a doubly-generic map with ngen and nmapConst *)
-
-Definition ngmap (n : nat) (k : kind) (t : ty k)
-  : kit k funTy (repeat (S n) (decodeClosed t)) :=
-  ngen t nmapConst.
-
-(*
-Definition ngeq (n : nat) (k : kind) (t : ty k)
-  : kit k geq (repeat (S n) (decodeClosed t)) :=
-  ngen t neqConst.
-      *)
-
-(* some test examples for map *)
-
-(* some test examples for unit map *)
-Compute ngmap 0 tunit. (* = () *)
-Compute ngmap 1 tunit tt. (* = () *)
-Compute ngmap 0 tnat. (* = 0 *)
-
-(* some test examples for nat map *)
-Compute ngmap 1 tnat 1. (* = 1 *)
-Compute ngmap 2 tnat 1 2. (* = 2 *)
-Compute ngmap 3 tnat 1 2 3. (* = 3 *)
-
-(* some test examples for prod map *)
-Compute ngmap 1 tprod nat nat
-  (fun x => x + 1) bool bool (fun _ => true) (1,true).
-Compute ngmap 2 tprod nat nat nat
-  (fun x y => x + y) bool bool bool (fun x y => andb x y) (1,true) (2, false).
-Compute ngmap 3 tprod nat nat nat nat
-  (fun x y z => x + y + z) bool bool nat nat
-  (fun x y z => if andb x y then 0 else z)
-  (1,true) (2, false) (1, 100). (* = (4, 100) *)
-
-(* some test examples for sum map *)
-Compute ngmap 1 tsum nat nat
-  (fun x => x + 1) bool bool (fun _ => true) (inl 1).
-Compute ngmap 2 tsum nat nat nat
-  (fun x y => x + y) bool bool bool (fun x y => andb x y)
-  (inl 1) (inl 1).
-Compute ngmap 3 tsum nat nat nat nat
-  (fun x y z => x + y + z) bool bool nat nat
-  (fun x y z => if andb x y then 0 else z)
-  (inr true) (inr false) (inr 4). (* = inr 4 *)
-
-(* some test examples for self defined maybe *)
-Compute ngmap 1 tmaybe _ bool (fun _ => false) (inl tt). (* = inl () *)
-Compute ngmap 2 tmaybe nat nat nat (fun x => fun y => x + y)
-  (inr 3) (inr 2).
-
-(*
-(* some test examples for unit eq *)
-Compute ngeq 0 tunit tt. (* = true *)
-Compute ngeq 1 tunit tt tt. (* = true *)
-
-(* some test examples for nat eq *)
-Compute ngeq 0 tnat 1. (* = true *)
-Compute ngeq 1 tnat 1 1. (* = true *)
-Compute ngeq 2 tnat 2 2 1. (* = false *)
-Compute ngeq 3 tnat 1 1 1 2. (* = false *)
-      *)
