examples.v
@@ -1,0 +1,316 @@
+Set Implicit Arguments.
+Set Universe Polymorphism.
+
+From Coq Require Import Program.
+
+Require Import generic univ utils.
+
+(* examples of defining types with the universe. *)
+Section univTypes.
+
+  (* Shorthands for constants *)
+  Definition tnat := Con nil Nat.
+  Definition tunit := Con nil Unit.
+  Definition tsum := Con nil Sum.
+  Definition tprod := Con nil Prod.
+
+  (* Shorthands for constants in a context *)
+  Definition tnatc := fun ctx => Con ctx Nat.
+  Definition tunitc := fun ctx => Con ctx Unit.
+  Definition tsumc := fun ctx => Con ctx Sum.
+  Definition tprodc := fun ctx => Con ctx Prod.
+
+  (* examples of defining maybe and either with the universe. *)
+
+  Definition tmaybe : ty (F Ty Ty) :=
+    Lam (App (App (tsumc _) (tunitc _)) (Var (Vz _ _))).
+
+  Definition teither : ty (F Ty (F Ty Ty)) :=
+    Lam (Lam
+      (App (App (tsumc _)
+        (Var (Vs _ (Vz _ _)))) (Var (Vz _ _)))).
+
+  (* Shorthands for decoding closed types *)
+  Definition deNat := decodeClosed (Con _ Nat).
+  Definition deUnit := decodeClosed (Con _ Unit).
+  Definition deMaybe (A : Set) := decodeClosed tmaybe A.
+  Definition deEither (A B : Set) := decodeClosed teither A B.
+
+  (* Compute examples *)
+  Compute deNat. (* = nat *)
+  Compute deUnit. (* = unit *)
+  Compute deMaybe. (* = fun A : Set => (unit + A) *)
+  Compute deMaybe nat. (* = (unit + nat) *)
+  Compute deEither. (* = fun A B : Set => (A + B) *)
+  Compute deEither nat unit. (* = (nat + unit) *)
+
+  Compute decodeClosed (Con _ Nat).
+
+End univTypes.
+
+(* Example of a datatype-generic function. *)
+Section dtgen.
+  (* type definition needed for gmap *)
+  Definition Map : vec Type 2 -> Type :=
+    fun vs => vhd vs -> vhd (vtl vs).
+
+  (* helper for defining sums *)
+  Definition doSum (A1 B1 : Type)
+    : (A1 -> B1) -> forall (A2 B2 : Type), (A2 -> B2) -> (A1 + A2) -> (B1 + B2) :=
+    fun f =>
+      fun _ _ g sa =>
+        match sa with
+        | inl a => inl (f a)
+        | inr b => inr (g b)
+        end.
+
+  (* helper for defining prods *)
+  Definition doProd (A1 B1 : Type)
+    : (A1 -> B1) -> forall (A2 B2 : Type), (A2 -> B2) -> (A1 * A2) -> (B1 * B2) :=
+    fun f _ _ g sa => (f (fst sa), g (snd sa)).
+
+  (** constants **)
+  Definition mapConst : tyConstEnv Map :=
+    fun k c =>
+      match c in const k
+      return kit k Map (repeat _ (decodeClosed (Con _ c)))
+      with
+      | Nat => fun n => n
+      | Unit => fun _ => tt
+      | Prod => doProd
+      | Sum => doSum
+      end.
+
+  (* gmap *)
+  Definition gmap (k : kind) (t : ty k) : kit k Map _ :=
+    ngen t mapConst.
+
+  (* examples  of using gmap *)
+  Compute gmap tprod nat nat (fun a => a + 1) bool bool (fun b => negb b) (1,true).
+  (* tmaybe is a self defined type, definition in 'univ.v' *)
+  Compute gmap tmaybe _ bool (fun _ => false) (inl tt). (* = inl () *)
+  Compute gmap tmaybe nat nat (fun n => n + 1) (inr 3). (* = inr 4 *)
+  (* teither is a self defined type, definition in 'univ.v' *)
+  Compute gmap teither _ bool (fun _ => false)
+                       _ bool (fun _ => true) (inl tt). (* = inl false *)
+
+End dtgen.
+
+(* Example of a arity-generic and datatype-generic function. *)
+Section aritydtgen.
+
+  (* type definition needed for doubly generic map *)
+  Fixpoint funTy {n : nat} (v : vec Type (S n)) : Type :=
+    match v with
+    | @vcons _ O x xs => x
+    | @vcons _ (S n') x xs => x -> funTy xs
+    end.
+
+  (* nat constant for nmapconst *)
+  Fixpoint cNat (n : nat) : kit Ty funTy (repeat (S n) _) :=
+    let f := (fix cNat' (n' : nat)
+      : kit Ty funTy (repeat (S n') nat) :=
+      match n' return kit Ty funTy (repeat (S n') nat) with
+      | O => O
+      | S O => fun x => x
+      | S (S m) => fun x y => cNat' m
+    end) in
+    match n return kit Ty funTy (repeat (S n) nat) with
+    | O => O
+    | S O => fun x => x
+    | (S (S m)) =>
+        if Nat.odd m
+        then fun x y => cNat m
+        else fun x => f (S m)
+    end.
+
+  (* unit constant for nmapconst *)
+  Fixpoint cUnit (n : nat) : kit Ty funTy (repeat (S n) _) :=
+    match n with
+    | O => tt
+    | S n' => fun x => cUnit n'
+    end.
+
+  (* Error axiom for finishing defs in sums *)
+  Axiom error : False.
+
+  (* helpers for defining sums *)
+  Fixpoint hSumLeft (n : nat)
+    : forall (va : vec Type (S n)), funTy va ->
+    forall (vb : vec Type (S n)), funTy (zap (zap (repeat _ sum) va) vb).
+  Proof.
+    intros VA a VB. simpl.
+    pose proof veq_hdtl VA as pfa;
+    pose proof veq_hdtl VB as pfb.
+    destruct n as [| n'].
+    - rewrite pfa in a. apply (inl a).
+    - intros x. destruct x.
+      + rewrite pfa in a. simpl in a.
+        pose proof a v as pa.
+        pose proof hSumLeft _ _ pa (vtl VB) as pf.
+        apply pf.
+      (* error case *)
+      + pose proof error as err. exfalso; apply err.
+  Defined.
+
+  Fixpoint hSumRight (n : nat)
+    : forall (va : vec Type (S n)) (vb : vec Type (S n)),
+    funTy vb -> funTy (zap (zap (repeat _ sum) va) vb).
+  Proof.
+    intros VA VB b. pose proof veq_hdtl VB as pfb.
+    destruct n as [| n'].
+    - rewrite pfb in b. apply (inr b).
+    - intros x; destruct x as [left | right].
+      (* error case *)
+      + exfalso; apply error.
+      + rewrite pfb in b. simpl in b.
+        pose proof b right as pb.
+        pose proof hSumRight n' (vtl VA)  (vtl VB) pb  as pf.
+        apply pf.
+  Defined.
+
+  Definition hSum (n : nat)
+    : forall (va : vec Type (S n)), funTy va
+    -> forall (vb : vec Type (S n)), funTy vb
+    -> funTy (zap (zap (repeat _ sum) va) vb).
+  Proof.
+    intros VA a VB b.
+    destruct n as [| n'].
+    (* no arguments, chooses arbitrary case inr *)
+    - simpl. rewrite veq_hdtl in b. simpl in b. apply (inr b).
+    - intros x; destruct x as [lr | rt].
+      + rewrite veq_hdtl in a. simpl in a.
+        pose proof a lr as pfa.
+        apply hSumLeft; apply pfa.
+      + rewrite veq_hdtl in b. simpl in b.
+        pose proof b rt as pfb.
+        apply hSumRight; apply pfb.
+ Defined.
+
+  (* sum constant for nmapconst *)
+  Definition cSum (n : nat) : kit (F Ty (F Ty Ty)) funTy (repeat (S n) sum).
+  Proof.
+  Admitted.
+
+  Program Fixpoint kindCurry (k : kind) (n : nat) (b : vec Type (S n) -> Type)
+    : forall v : vec (decodeKind k) (S n),
+    unkit k b v -> kit k b v :=
+    match k
+    return forall v : vec (decodeKind k) (S n),
+    unkit k b v -> kit k b v
+    with
+    | Ty => _
+    | F k1 k2 => fun v vs =>
+        curry (fun (x:vec (decodeKind k1) _) =>
+              kit k1 b x ->
+              kit k2 b (zap v x))
+              (fun As y => kindCurry k2 _ (zap v As) (vs As y))
+    end.
+
+  (* helper for defining prods *)
+  Fixpoint hProd (n : nat)
+    : forall (va : vec Type (S n)), funTy va
+    -> forall (vb : vec Type (S n)), funTy vb
+    -> funTy (zap (zap (repeat _ prod) va) vb).
+      Proof.
+        destruct n;
+        intros VA a VB b;
+        pose proof veq_hdtl VA as pfa;
+        pose proof veq_hdtl VB as pfb.
+        - apply pair.
+          + rewrite pfa in a; apply a.
+          + rewrite pfb in b; apply b.
+        - refine (fun pr => _). intros.
+          destruct pr as [pa pb].
+          apply hProd.
+          + rewrite pfa in a. apply a. apply pa.
+          + rewrite pfb in b. apply b. apply pb.
+      Defined.
+
+  (* prod constant for nmapconst *)
+  Fixpoint cProd (n : nat) : kit (F Ty (F Ty Ty)) funTy (repeat (S n) prod).
+  Proof.
+    apply (kindCurry (F Ty (F Ty Ty))).
+    simpl. intros VA a VB b.
+    pose proof hProd VA a VB b as hp.
+    simpl in hp.
+    apply hp.
+  Defined.
+
+  Fixpoint nmapConst {n : nat} : tyConstEnv (@funTy n).
+  refine (fun k c => _).
+  refine
+  (match c with
+    | Nat => _
+    | Unit => _
+    | Prod => _
+    | Sum => _
+    end
+  ).
+  (* CASE FOR NAT
+    this just returns 0 for all,
+     maybe change to return last nat given (like cNat) *)
+  - induction n.
+    + simpl. apply (cNat 0).
+    + refine (fun x => _). apply IHn.
+  (* CASE FOR UNIT *)
+  - induction n.
+    + apply tt.
+    + refine (fun x => _). apply IHn.
+  (* CASE FOR SUM *)
+  - pose proof (kindCurry (F Ty (F Ty Ty))) as pf.
+    apply pf. simpl. intros VA a VB b.
+    pose proof hSum VA a VB b as hp. simpl in hp.
+    apply hp.
+  (* CASE FOR PROD *)
+  - pose proof (kindCurry (F Ty (F Ty Ty))) as pf.
+    apply pf. simpl. intros VA a VB b.
+    pose proof hProd VA a VB b as hp. simpl in hp.
+    apply hp.
+  Defined.
+
+
+  (* doubly generic map *)
+  Definition ngmap (n : nat) (k : kind) (t : ty k)
+    : kit k funTy (repeat (S n) (decodeClosed t)) :=
+    ngen t nmapConst.
+
+  (* some test examples for unit map *)
+  Compute ngmap 0 tunit. (* = () *)
+  Compute ngmap 1 tunit tt. (* = () *)
+  Compute ngmap 0 tnat. (* = 0 *)
+
+  (* some test examples for nat map *)
+  Compute ngmap 1 tnat 1. (* = 1 *)
+  Compute ngmap 2 tnat 1 2. (* = 2 *)
+  Compute ngmap 3 tnat 1 2 3. (* = 3 *)
+
+  (* some test examples for prod map *)
+  Compute ngmap 1 tprod _ _
+    (fun x => x + 1) _ _ (fun _ => true) (1,false).
+  Compute ngmap 2 tprod nat nat nat
+    (fun x y => x + y) bool bool bool (fun x y => andb x y) (1,true) (2, false).
+  Compute ngmap 3 tprod nat nat nat nat
+    (fun x y z => x + y + z) bool bool nat nat
+    (fun x y z => if andb x y then 0 else z)
+    (1,true) (2, false) (1, 100). (* = (4, 100) *)
+
+  (* some test examples for sum map *)
+  Compute ngmap 1 tsum
+    _ _ (fun x => x + 1)
+    _ _ (fun _ => true)
+    (inl 1). (* = inl 2 *)
+  Compute ngmap 2 tsum nat nat nat
+    (fun x y => x + y) bool bool bool (fun x y => andb x y)
+    (inl 1) (inl 1).
+  Compute ngmap 3 tsum nat nat nat nat
+    (fun x y z => x + y + z) bool bool nat nat
+    (fun x y z => if andb x y then 0 else z)
+    (inr true) (inr false) (inr 4). (* = inr 4 *)
+
+  (* some test examples for self defined tmaybe *)
+  Compute ngmap 1 tmaybe _ bool (fun _ => false) (inl tt). (* = inl () *)
+  Compute ngmap 2 tmaybe nat nat nat (fun x => fun y => x + y)
+    (inr 3) (inr 2).
+
+End aritydtgen.
