proofs.v
@@ -1,0 +1,24 @@
+Set Implicit Arguments.
+
+Require Import univ utils.
+
+(* A few example proofs with the universe. *)
+
+(* Decoding constants in a closed env always correct. *)
+
+Theorem natdeceq :
+  decodeClosed (Con nil Nat) = nat.
+Proof. unfold decodeClosed; unfold decodeType. reflexivity. Defined.
+
+Theorem unitdeceq :
+  decodeClosed (Con nil Unit) = unit.
+Proof. unfold decodeClosed; unfold decodeType. reflexivity. Defined.
+
+Theorem prdeceq :
+  decodeClosed (Con nil Prod) = prod.
+Proof. unfold decodeClosed; unfold decodeType. reflexivity. Defined.
+
+Theorem smdeceq :
+  decodeClosed (Con nil Sum) = sum.
+Proof. unfold decodeClosed; unfold decodeType. reflexivity. Defined.
+
