Makefile
@@ -7,6 +7,8 @@ all:
 	coqc arity.v
 	coqc $(args) univ.v
 	coqc $(args) generic.v
+	coqc $(args) examples.v
+	coqc $(args) proofs.v
 
 clean:
 	rm *.vok *.glob *.vo *.vos
